bedrock2/src/bedrock2/ZnWordsTests.v
@@ -1,0 +1,24 @@
+Require Import Coq.ZArith.ZArith. Open Scope Z_scope.
+Require Import bedrock2.ZnWords.
+Require Import coqutil.Word.Interface.
+
+Section ZnWordTests.
+  Context {word: word.word 32} {word_ok: word.ok word}.
+
+  Goal forall (a a' SZ: word) (T: Type) (f: T -> nat) (vs1: T),
+      word.unsigned (word.sub a' a) mod word.unsigned SZ = 0 ->
+      f vs1 = Z.to_nat (word.unsigned (word.sub a' a) / word.unsigned SZ) ->
+      word.add a (word.of_Z (word.unsigned (word.of_Z (word := word) (word.unsigned SZ))
+                             * Z.of_nat (f vs1))) = a'.
+  Proof.
+    intros.
+    Fail ZnWords.
+    (* This rewrite should not be needed, but it seems to be a limitation of lia:
+       https://github.com/coq/coq/issues/15583
+       TODO remove the rewrite if lia is fixed. *)
+    rewrite H0.
+    ZnWords.
+    all: fail "remaining subgoals".
+  Abort.
+
+End ZnWordTests.
